Garden/Halo2/halo2_gadgets/utilities/lookup_range_check_proof.v
@@ -93,7 +93,8 @@ Module RangeTable.
       Γ.(Assignment.lookup) table_idx i = i.
     Proof.
       cbn [interpret_fact] in Hfact.
-      rewrite Hfact by lia.
+      rewrite Hfact by
+        (rewrite List.length_map, List.length_seq, Z2Nat.id by lia; lia).
       unfold value_at_row.
       rewrite nth_map_seq by (apply Z2Nat.inj_lt; lia).
       apply Z2Nat.id; lia.
